Prove captureNext correctness

RegexCorrectness/NFA/VM/Traversal.lean
@@ -1,2 +1,216 @@
 -- Correctness of the graph traversal implementation
+import Regex.NFA.VM.Basic
 import RegexCorrectness.NFA.VM.Traversal.Aux
+
+open NFA.VM
+
+/--
+Increment the end position by one character.
+-/
+def Substring.expand (s : Substring) : Substring :=
+  if s.stopPos < s.str.endPos then
+    { s with stopPos := s.str.next s.stopPos }
+  else
+    s
+
+namespace Substring.ValidFor
+
+theorem expand (v : ValidFor l m (c :: r) s) : ValidFor l (m ++ [c]) r s.expand := by
+  simp [Substring.expand, v.stopPos, v.str, String.csize_pos, String.next]
+  have : String.get ⟨l ++ (m ++ c :: r)⟩ ⟨String.utf8Len l + String.utf8Len m⟩ = c := by
+    have eq₁ : l ++ (m ++ c :: r) = (l ++ m) ++ (c :: r) := by simp
+    have eq₂ : String.utf8Len l + String.utf8Len m = String.utf8Len (l ++ m) := by simp
+    rw [eq₁, eq₂, String.get_of_valid]
+    simp
+  rw [this]
+
+  apply of_eq
+  . simp
+  . simp [v.startPos]
+  . simp [Nat.add_assoc]
+
+end Substring.ValidFor
+
+namespace String.Iterator.Valid
+
+theorem next' {it : Iterator} (v : it.Valid) (h : ¬it.atEnd) : it.next.Valid := by
+  apply v.next
+  simp [hasNext, atEnd] at *
+  exact h
+
+end String.Iterator.Valid
+
+namespace String.Iterator.ValidFor
+
+theorem exists_cons_of_not_atEnd {it : Iterator} (v : it.ValidFor l r) (h : ¬it.atEnd) :
+  ∃ r', r = it.curr :: r' := by
+  have := v.atEnd
+  simp [h] at this
+  have ⟨c, r', heq⟩ := List.exists_cons_of_ne_nil this
+  subst heq
+  have := v.curr
+  simp at this
+  subst this
+  exact ⟨r', rfl⟩
+
+end String.Iterator.ValidFor
+
+namespace NFA
+
+/--
+`nfa.reaches i cs` means that there is a path from the start node to `i` given by interleaving
+ε closures and character steps, which corresponds to `cs`.
+-/
+inductive reaches (nfa : NFA) : Fin nfa.nodes.size → List Char → Prop where
+  | nil (cls : i.val ∈ nfa.εClosure nfa.start) : nfa.reaches i []
+  | snoc {i : Fin nfa.nodes.size} {j : Nat} {c : Char} {cs : List Char}
+    (prev : reaches nfa i cs) (step : j ∈ nfa.charStep i c) (cls : k.val ∈ nfa.εClosure j) :
+    nfa.reaches k (cs ++ [c])
+
+structure captureNext.go.Inv (nfa : NFA) (it : String.Iterator)
+  (current : SparseSet nfa.nodes.size) (lastMatch : Option (Array (Option String.Pos))) where
+  currentClosure : ∀ i j : Fin nfa.nodes.size, i ∈ current → j.val ∈ nfa.εStep i → j ∈ current
+  -- For all states in `current`, there is a path from `nfa.start` to it, the match starting at `l`.
+  -- The matching substring corresponds to `m`, and `r` denotes the remaining input.
+  currentPath : ∀ i, i ∈ current → ∃ (s : Substring) (l m r : List Char),
+    s.ValidFor l m r ∧ it.ValidFor (m.reverse ++ l.reverse) r ∧ nfa.reaches i m
+  acceptOfLastMatch : lastMatch.isSome → ∃ (s : Substring) (l m r : List Char),
+    s.ValidFor l m r ∧ ∃ i, nfa.reaches i m ∧ nfa[i] = .done
+
+-- TODO: to be precise, we should associate the substring `s` with the underlying string of `it`
+theorem captureNext_spec.go
+  (h : captureNext.go nfa saveSize it current next saveSlots lastMatch = matched)
+  (inv : captureNext.go.Inv nfa it current lastMatch)
+  (v : it.Valid)
+  (hemp : next.isEmpty) :
+  matched.isSome → ∃ (s : Substring) (l m r : List Char),
+    s.ValidFor l m r ∧ ∃ i, nfa.reaches i m ∧ nfa[i] = .done := by
+  unfold captureNext.go at h
+  split at h
+  next =>
+    subst h
+    exact inv.acceptOfLastMatch
+  next atEnd =>
+    split at h
+    next h' =>
+      subst h
+      exact inv.acceptOfLastMatch
+    next =>
+      if hm : lastMatch.isNone then
+        generalize he : exploreεClosure nfa it.pos current (captureNext.initSave saveSize) none saveSlots nfa.start #[] = explored at h
+        let (_, current', saveSlots') := explored
+        simp [hm] at h
+        have mem_current'_iff := exploreεClosure_spec.mem_next_iff he inv.currentClosure
+
+        generalize hs : eachStepChar nfa it.curr it.next.pos current' next saveSlots' = stepped at h
+        let (matched', next', saveSlots'') := stepped
+        simp at h
+
+        have currentPath'  (k : Fin nfa.nodes.size) (hk : k ∈ next') :
+          ∃ (s : Substring) (l m r : List Char), s.ValidFor l m r ∧ it.next.ValidFor (m.reverse ++ l.reverse) r ∧ nfa.reaches k m := by
+          have ⟨_, mem_next_iff⟩ := eachStepChar_spec.mem_next_iff hs hemp
+          have ⟨i, isLt, _, ⟨j, step, cls⟩⟩ := (mem_next_iff k).mp hk
+          cases (mem_current'_iff current'[i]).mp (SparseSet.mem_get isLt) with
+          | inl mem_current =>
+            -- Previous search continues
+            have ⟨s, l, m, r, sv, iv, prev⟩ := inv.currentPath current'[i] mem_current
+            have ⟨r', hr⟩ := iv.exists_cons_of_not_atEnd atEnd
+            subst hr
+            exact ⟨s.expand, l, m ++ [it.curr], r', sv.expand, by simp [iv.next], prev.snoc step cls⟩
+          | inr cls' =>
+            -- New search from `it.pos`
+            have ⟨l, r, iv⟩ := v.validFor
+            have ⟨r', hr⟩ := iv.exists_cons_of_not_atEnd atEnd
+            subst hr
+            let startPos : String.Pos := ⟨String.utf8Len l⟩
+            refine ⟨⟨it.toString, startPos, startPos + it.curr⟩, l.reverse, [it.curr], r', ?_, ?_, ?_⟩
+            . apply Substring.ValidFor.of_eq <;> simp [iv.toString, List.reverseAux_eq]
+            . apply String.Iterator.ValidFor.of_eq <;> simp [iv.next.toString, iv.next.pos]
+            . have prev : nfa.reaches current'[i] [] := .nil cls'
+              exact prev.snoc step cls
+
+        have acceptOfLastMatch' (h : (matched' <|> lastMatch).isSome) :
+          ∃ (s : Substring) (l m r : List Char), s.ValidFor l m r ∧ ∃ i, nfa.reaches i m ∧ nfa[i] = .done := by
+          cases matched' with
+          | none =>
+            simp at h
+            exact inv.acceptOfLastMatch h
+          | some =>
+            have ⟨i, hi, hdone⟩ := (eachStepChar_spec.mem_done_iff hs hemp).mpr rfl
+            have ⟨s, l, m, r, sv, _, reaches⟩ := currentPath' i hi
+            exact ⟨s, l, m, r, sv, ⟨i, reaches, hdone⟩⟩
+
+        have inv' : captureNext.go.Inv nfa it.next next' (matched' <|> lastMatch) :=
+          ⟨eachStepChar_spec.preserve_cls hs hemp, currentPath', acceptOfLastMatch'⟩
+        exact captureNext_spec.go h inv' (v.next' atEnd) (by simp)
+      else
+        simp [hm] at h
+
+        generalize hs : eachStepChar nfa it.curr it.next.pos current next saveSlots = stepped at h
+        let (matched', next', saveSlots'') := stepped
+        simp at h
+
+        have currentPath' (k : Fin nfa.nodes.size) (hk : k ∈ next') :
+          ∃ (s : Substring) (l m r : List Char), s.ValidFor l m r ∧ it.next.ValidFor (m.reverse ++ l.reverse) r ∧ nfa.reaches k m := by
+          have ⟨_, mem_next_iff⟩ := eachStepChar_spec.mem_next_iff hs hemp
+          have ⟨i, isLt, _, ⟨j, step, cls⟩⟩ := (mem_next_iff k).mp hk
+          have ⟨s, l, m, r, sv, iv, prev⟩ := inv.currentPath current[i] (SparseSet.mem_get isLt)
+          have ⟨r', hr⟩ := iv.exists_cons_of_not_atEnd atEnd
+          subst hr
+          exact ⟨s.expand, l, m ++ [it.curr], r', sv.expand, by simp [iv.next], prev.snoc step cls⟩
+
+        have acceptOfLastMatch' (h : (matched' <|> lastMatch).isSome) :
+          ∃ (s : Substring) (l m r : List Char), s.ValidFor l m r ∧ ∃ i, nfa.reaches i m ∧ nfa[i] = .done := by
+          cases matched' with
+          | none =>
+            simp at h
+            exact inv.acceptOfLastMatch h
+          | some =>
+            have ⟨i, hi, hdone⟩ := (eachStepChar_spec.mem_done_iff hs hemp).mpr rfl
+            have ⟨s, l, m, r, sv, _, reaches⟩ := currentPath' i hi
+            exact ⟨s, l, m, r, sv, ⟨i, reaches, hdone⟩⟩
+
+        have inv' : captureNext.go.Inv nfa it.next next' (matched' <|> lastMatch) :=
+          ⟨eachStepChar_spec.preserve_cls hs hemp, currentPath', acceptOfLastMatch'⟩
+        exact captureNext_spec.go h inv' (v.next' atEnd) (by simp)
+
+theorem captureNext_spec
+  (h : captureNext nfa it saveSize = matched)
+  (v : it.Valid)
+  (hsome : matched.isSome) :
+  ∃ (s : Substring) (l m r : List Char),
+    s.ValidFor l m r ∧ ∃ i, nfa.reaches i m ∧ nfa[i] = .done := by
+  unfold captureNext at h
+  generalize _hs : Vec.ofFn (fun _ => captureNext.initSave saveSize) = saveSlots at h
+  simp at h
+  generalize he : exploreεClosure nfa it.pos .empty (captureNext.initSave saveSize) .none saveSlots nfa.start #[] = init at h
+  let (matched', init', saveSlots) := init
+  simp at h
+
+  have hnotMem (i : Fin nfa.nodes.size) : ¬i ∈ SparseSet.empty := by
+    simp only [SparseSet.not_mem_of_isEmpty SparseSet.isEmpty_empty]
+    simp
+
+  have inv : captureNext.go.Inv nfa it init' matched' := by
+    refine ⟨exploreεClosure_spec.preserve_cls he (by simp only [hnotMem]; simp), ?_, ?_⟩
+    . intro i hi
+      have ⟨l, r, v'⟩ := v.validFor
+      let pos : String.Pos := ⟨String.utf8Len l⟩
+      refine ⟨⟨it.toString, pos, pos⟩, l.reverse, [], r, ?_, by simp [v'], .nil ?_⟩
+      . apply Substring.ValidFor.of_eq <;> simp [v'.toString, List.reverseAux_eq]
+      . have := (exploreεClosure_spec.mem_next_iff he (by simp only [hnotMem]; simp) i).mp hi
+        simp only [hnotMem] at this
+        simp at this
+        exact this
+    . intro hsome
+      have ⟨i, hi, hdone⟩ := (exploreεClosure_mem_done_iff he (by simp only [hnotMem]; simp)).mpr hsome
+      have cls := (exploreεClosure_spec.mem_next_iff he (by simp only [hnotMem]; simp) i).mp hi
+      simp only [hnotMem] at cls
+      simp at cls
+      have ⟨l, r, v'⟩ := v.validFor
+      let pos : String.Pos := ⟨String.utf8Len l⟩
+      refine ⟨⟨it.toString, pos, pos⟩, l.reverse, [], r, ?_, ⟨i, .nil cls, hdone⟩⟩
+      apply Substring.ValidFor.of_eq <;> simp [v'.toString, List.reverseAux_eq]
+  exact captureNext_spec.go h inv v (by simp) hsome
+
+end NFA
